Completed (half of) TCO

05TreeCode/TailCallOptimization.thy
@@ -2,106 +2,178 @@ theory TailCallOptimization
   imports TreeCode "../00Utils/Iteration"
 begin
 
+fun tco_r :: "tree_code list \<Rightarrow> tree_return" where
+  "tco_r [] = TReturn"
+| "tco_r (TApply # cd) = (case cd of 
+      [] \<Rightarrow> TJump
+    | _ \<Rightarrow> tco_r cd)"
+| "tco_r (op # cd) = tco_r cd"
+
 fun tco :: "tree_code list \<Rightarrow> tree_code list" where
   "tco [] = []"
-| "tco (TApply # TReturn # cd) = TJump # tco cd"
-| "tco (TPushLam cd' # cd) = TPushLam (tco cd') # tco cd"
+| "tco (TApply # cd) = (case cd of 
+      [] \<Rightarrow> []
+    | _ \<Rightarrow> TApply # tco cd)"
+| "tco (TPushLam cd' r # cd) = TPushLam (tco cd') (tco_r cd') # tco cd"
 | "tco (op # cd) = op # tco cd"
 
 primrec tco_val :: "tclosure \<Rightarrow> tclosure" where
   "tco_val (TConst k) = TConst k"
-| "tco_val (TLam t cd) = TLam t (tco cd)"
+| "tco_val (TLam vs cd r) = TLam (map tco_val vs) (tco cd) (tco_r cd)"
+
+fun tco_stack_frame :: "tree_stack_frame \<Rightarrow> tree_stack_frame" where
+  "tco_stack_frame (vs, cd, r) = (map tco_val vs, tco cd, tco_r cd)"
+
+fun not_dead_frame :: "tree_stack_frame \<Rightarrow> bool" where
+  "not_dead_frame (vs, cd, r) = (cd \<noteq> [] \<or> r \<noteq> TReturn)"
+
+abbreviation tco_stack :: "tree_stack_frame list \<Rightarrow> tree_stack_frame list" where
+  "tco_stack sfs \<equiv> filter not_dead_frame (map tco_stack_frame sfs)"
 
 primrec tco_state :: "tree_code_state \<Rightarrow> tree_code_state" where
-  "tco_state (TS vs envs cd) = TS (map tco_val vs) (map (map tco_val) envs) (tco cd)"
+  "tco_state (TS vs sfs) = TS (map tco_val vs) (tco_stack sfs)"
 
-fun untco :: "tree_code list \<Rightarrow> tree_code list" where
-  "untco [] = []"
-| "untco (TJump # cd) = TApply # TReturn # untco cd"
-| "untco (TPushLam cd' # cd) = TPushLam (untco cd') # untco cd"
-| "untco (op # cd) = op # untco cd"
+fun jump_free_code :: "tree_code list \<Rightarrow> bool" where
+  "jump_free_code [] = True"
+| "jump_free_code (TPushLam cd' r # cd) = (jump_free_code cd' \<and> r \<noteq> TJump \<and> jump_free_code cd)"
+| "jump_free_code (op # cd) = jump_free_code cd"
 
-primrec untco_val :: "tclosure \<Rightarrow> tclosure" where
-  "untco_val (TConst k) = TConst k"
-| "untco_val (TLam t cd) = TLam t (untco cd)"
+primrec jump_free_val :: "tclosure \<Rightarrow> bool" where
+  "jump_free_val (TConst k) = True"
+| "jump_free_val (TLam t cd r) =  (jump_free_code cd \<and> r \<noteq> TJump)"
 
-primrec untco_state :: "tree_code_state \<Rightarrow> tree_code_state" where
-  "untco_state (TS vs envs cd) = TS (map untco_val vs) (map (map untco_val) envs) (untco cd)"
+fun jump_free_frame :: "tree_stack_frame \<Rightarrow> bool" where
+  "jump_free_frame (vs, cd, r) =  (list_all jump_free_val vs \<and> jump_free_code cd \<and> r \<noteq> TJump)"
 
-fun no_jumps :: "tree_code list \<Rightarrow> bool" where
-  "no_jumps [] = True"
-| "no_jumps (TJump # cd) = False"
-| "no_jumps (TPushLam cd' # cd) = (no_jumps cd' \<and> no_jumps cd)"
-| "no_jumps (op # cd) = no_jumps cd"
-
-primrec no_jumps_val :: "tclosure \<Rightarrow> bool" where
-  "no_jumps_val (TConst k) = True"
-| "no_jumps_val (TLam t cd) = no_jumps cd"
-
-primrec no_jumps_state :: "tree_code_state \<Rightarrow> bool" where
-  "no_jumps_state (TS vs envs cd) = 
-    (list_all no_jumps_val vs \<and> list_all (list_all no_jumps_val) envs \<and> no_jumps cd)"
-
-fun no_unjumps :: "tree_code list \<Rightarrow> bool" where
-  "no_unjumps [] = True"
-| "no_unjumps (TApply # TReturn # cd) = False"
-| "no_unjumps (TPushLam cd' # cd) = (no_unjumps cd' \<and> no_unjumps cd)"
-| "no_unjumps (op # cd) = no_unjumps cd"
-
-primrec no_unjumps_val :: "tclosure \<Rightarrow> bool" where
-  "no_unjumps_val (TConst k) = True"
-| "no_unjumps_val (TLam t cd) = no_unjumps cd"
-
-primrec no_unjumps_state :: "tree_code_state \<Rightarrow> bool" where
-  "no_unjumps_state (TS vs envs cd) = 
-    (list_all no_unjumps_val vs \<and> list_all (list_all no_unjumps_val) envs \<and> no_unjumps cd)"
-
-lemma [simp]: "no_unjumps (tco cd)"
-proof (induction cd rule: tco.induct)
-  case ("4_27" cd)
-  thus ?case by (cases cd rule: tco.cases) simp_all
-qed simp_all
-
-lemma [simp]: "no_jumps (untco cd)"
-  by (induction cd rule: tco.induct) simp_all
-
-lemma [simp]: "no_jumps cd \<Longrightarrow> untco (tco cd) = cd"
-  by (induction cd rule: tco.induct) simp_all
-
-lemma [simp]: "no_jumps_val v \<Longrightarrow> untco_val (tco_val v) = v"
-  by (induction v) simp_all
-
-lemma [simp]: "list_all no_jumps_val vs \<Longrightarrow> map (untco_val \<circ> tco_val) vs = vs"
-  by (induction vs) simp_all
-
-lemma [simp]: "list_all (list_all no_jumps_val) vss \<Longrightarrow> map (map (untco_val \<circ> tco_val)) vss = vss"
-  by (induction vss) simp_all
-
-lemma [simp]: "no_jumps_state \<Sigma> \<Longrightarrow> untco_state (tco_state \<Sigma>) = \<Sigma>"
-  by (induction \<Sigma>) simp_all
-
-lemma [simp]: "no_unjumps cd \<Longrightarrow> tco (untco cd) = cd"
-  by (induction cd rule: tco.induct) simp_all
-
-lemma [simp]: "no_unjumps_val v \<Longrightarrow> tco_val (untco_val v) = v"
-  by (induction v) simp_all
-
-lemma [simp]: "list_all no_unjumps_val vs \<Longrightarrow> map (tco_val \<circ> untco_val) vs = vs"
-  by (induction vs) simp_all
-
-lemma [simp]: "list_all (list_all no_unjumps_val) vss \<Longrightarrow> map (map (tco_val \<circ> untco_val)) vss = vss"
-  by (induction vss) simp_all
-
-lemma [simp]: "no_unjumps_state \<Sigma> \<Longrightarrow> tco_state (untco_state \<Sigma>) = \<Sigma>"
-  by (induction \<Sigma>) simp_all
-
-theorem correcttco [simp]: "\<Sigma> \<leadsto>\<^sub>t \<Sigma>' \<Longrightarrow> tco_state \<Sigma> \<leadsto>\<^sub>t tco_state \<Sigma>'"
-  by simp
+primrec jump_free_state :: "tree_code_state \<Rightarrow> bool" where
+  "jump_free_state (TS vs sfs) = (list_all jump_free_val vs \<and> list_all jump_free_frame sfs)"
 
 theorem completetco [simp]: "tco_state \<Sigma> \<leadsto>\<^sub>t \<Sigma>' \<Longrightarrow> \<exists>\<Sigma>''. \<Sigma> \<leadsto>\<^sub>t \<Sigma>'' \<and> \<Sigma>' = tco_state \<Sigma>''"
   by simp
 
-lemma iter_tco_eval [simp]: "iter (\<leadsto>\<^sub>t) \<Sigma> \<Sigma>' \<Longrightarrow> iter (\<leadsto>\<^sub>t) (tco_state \<Sigma>) (tco_state \<Sigma>')"
-  by (induction \<Sigma> \<Sigma>' rule: iter.induct) (simp, metis iter_step correcttco)
+lemma [simp]: "tco (op # cd) = [] \<Longrightarrow> tco_r (op # cd) = TJump"
+  by (induction op) (simp_all split: list.splits)
+
+lemma tco_never_dead [simp]: "not_dead_frame (vs, tco (op # cd), tco_r (op # cd))"
+  by (induction cd rule: tco.induct) (simp_all split: list.splits)
+
+lemma jump_free_persists [simp]: "\<Sigma> \<leadsto>\<^sub>t \<Sigma>' \<Longrightarrow> jump_free_state \<Sigma> \<Longrightarrow> jump_free_state \<Sigma>'"
+  by (induction \<Sigma> \<Sigma>' rule: evalt.induct) auto
+
+theorem correcttco [simp]: "\<Sigma> \<leadsto>\<^sub>t \<Sigma>' \<Longrightarrow> jump_free_state \<Sigma> \<Longrightarrow> 
+  iter (\<leadsto>\<^sub>t) (tco_state \<Sigma>) (tco_state \<Sigma>')"
+proof (induction \<Sigma> \<Sigma>' rule: evalt.induct)
+  case (evt_lookup env x v vs cd r sfs)
+  thus ?case 
+  proof (cases cd)
+    case Nil
+    from evt_lookup have "tco_state (TS vs ((env, [TLookup x], r) # sfs)) \<leadsto>\<^sub>t
+      TS (tco_val v # map tco_val vs) ((map tco_val env, [], TReturn) # tco_stack sfs)" by simp
+    moreover have "TS (tco_val v # map tco_val vs) ((map tco_val env, [], TReturn) # tco_stack sfs)
+      \<leadsto>\<^sub>t tco_state (TS (v # vs) ((env, [], r) # sfs))" by simp
+    ultimately have "iter (\<leadsto>\<^sub>t) (tco_state (TS vs ((env, [TLookup x], r) # sfs)))
+      (tco_state (TS (v # vs) ((env, [], r) # sfs)))" by (metis iter_refl iter_step)
+    with Nil show ?thesis by simp
+  next
+    case (Cons op cd)
+    moreover from evt_lookup have "tco_state (TS vs ((env, TLookup x # op # cd, r) # sfs)) \<leadsto>\<^sub>t
+      tco_state (TS (v # vs) ((env, op # cd, r) # sfs))" by simp
+    ultimately show ?thesis by (metis iter_one)
+  qed
+next
+  case (evt_pushcon vs env k cd r sfs)
+  thus ?case 
+  proof (cases cd)
+    case Nil
+    have "tco_state (TS vs ((env, [TPushCon k], r) # sfs)) \<leadsto>\<^sub>t
+      TS (TConst k # map tco_val vs) ((map tco_val env, [], TReturn) # tco_stack sfs)" by simp
+    moreover have "TS (TConst k # map tco_val vs) ((map tco_val env, [], TReturn) # tco_stack sfs)
+      \<leadsto>\<^sub>t tco_state (TS (TConst k # vs) ((env, [], r) # sfs))" by simp
+    ultimately have "iter (\<leadsto>\<^sub>t) (tco_state (TS vs ((env, [TPushCon k], r) # sfs)))
+      (tco_state (TS (TConst k # vs) ((env, [], r) # sfs)))" by (metis iter_refl iter_step)
+    with Nil show ?thesis by simp
+  next
+    case (Cons op cd)
+    moreover from evt_lookup have "tco_state (TS vs ((env, TPushCon k # op # cd, r) # sfs)) \<leadsto>\<^sub>t
+      tco_state (TS (TConst k # vs) ((env, op # cd, r) # sfs))" by simp
+    ultimately show ?thesis by (metis iter_one)
+  qed
+next
+  case (evt_pushlam vs env cd' r' cd r sfs)
+  thus ?case 
+  proof (cases cd)
+    case Nil
+    have "tco_state (TS vs ((env, [TPushLam cd' r'], r) # sfs)) \<leadsto>\<^sub>t
+      TS (TLam (map tco_val env) (tco cd') (tco_r cd') # map tco_val vs) 
+        ((map tco_val env, [], TReturn) # tco_stack sfs)" by simp
+    moreover have "TS (TLam (map tco_val env) (tco cd') (tco_r cd') # map tco_val vs) 
+      ((map tco_val env, [], TReturn) # tco_stack sfs) \<leadsto>\<^sub>t 
+        tco_state (TS (TLam env cd' r' # vs) ((env, [], r) # sfs))" by simp
+    ultimately have "iter (\<leadsto>\<^sub>t) (tco_state (TS vs ((env, [TPushLam cd' r'], r) # sfs)))
+      (tco_state (TS (TLam env cd' r' # vs) ((env, [], r) # sfs)))" by (metis iter_refl iter_step)
+    with Nil show ?thesis by simp
+  next
+    case (Cons op cd)
+    moreover from evt_lookup have "tco_state (TS vs ((env, TPushLam cd' r' # op # cd, r) # sfs)) \<leadsto>\<^sub>t
+      tco_state (TS (TLam env cd' r' # vs) ((env, op # cd, r) # sfs))" by simp
+    ultimately show ?thesis by (metis iter_one)
+  qed
+next
+  case (evt_apply v env cd' r' vs cd r sfs)
+  thus ?case 
+  proof (cases cd)
+    case Nil note CD = Nil
+    thus ?thesis
+    proof (cases cd')
+      case Nil
+      have "TS (map tco_val vs) ((tco_val v # map tco_val env, [], TReturn) # tco_stack sfs) \<leadsto>\<^sub>t
+          tco_state (TS vs ((v # env, [], r') # (env, [], r) # sfs))" by simp
+      hence "iter (\<leadsto>\<^sub>t) (TS (map tco_val vs) 
+        ((tco_val v # map tco_val env, [], TReturn) # tco_stack sfs))
+          (tco_state (TS vs ((v # env, [], r') # (env, [], r) # sfs)))" by (metis iter_one)
+      moreover have "tco_state (TS (v # TLam env [] r' # vs) ((env, [TApply], r) # sfs)) \<leadsto>\<^sub>t
+          TS (map tco_val vs) ((tco_val v # map tco_val env, [], TReturn) # tco_stack sfs)" by simp
+      ultimately have "iter (\<leadsto>\<^sub>t) (tco_state (TS (v # TLam env [] r' # vs) 
+        ((env, [TApply], r) # sfs)))
+          (tco_state (TS vs ((v # env, [], r') # (env, [], r) # sfs)))" using iter_step by fast
+      with CD Nil show ?thesis by simp
+    next
+      case (Cons op' cd')
+      have "tco_state (TS (v # TLam env (op' # cd') r' # vs) ((env, [TApply], r) # sfs)) \<leadsto>\<^sub>t
+        tco_state (TS vs ((v # env, op' # cd', r') # (env, [], r) # sfs))" by simp
+      with Nil Cons show ?thesis by (metis iter_one)
+    qed
+  next
+    case (Cons op cd) note CD = Cons
+    thus ?thesis
+    proof (cases cd')
+      case Nil
+      have "TS (map tco_val vs) ((tco_val v # map tco_val env, [], TReturn) # 
+        (map tco_val env, tco (op # cd), tco_r (op # cd)) # tco_stack sfs) \<leadsto>\<^sub>t
+          tco_state (TS vs ((v # env, [], r') # (env, op # cd, r) # sfs))" by simp
+      hence "iter (\<leadsto>\<^sub>t) (TS (map tco_val vs) ((tco_val v # map tco_val env, [], TReturn) # 
+        (map tco_val env, tco (op # cd), tco_r (op # cd)) # tco_stack sfs)) 
+          (tco_state (TS vs ((v # env, [], r') # (env, op # cd, r) # sfs)))" by (metis iter_one)
+      moreover have "tco_state (TS (v # TLam env [] r' # vs) ((env, TApply # op # cd, r) # sfs)) \<leadsto>\<^sub>t
+        TS (map tco_val vs) ((tco_val v # map tco_val env, [], TReturn) # 
+          (map tco_val env, tco (op # cd), tco_r (op # cd)) # tco_stack sfs)" by simp
+      ultimately have "iter (\<leadsto>\<^sub>t) (tco_state (TS (v # TLam env [] r' # vs) 
+        ((env, TApply # op # cd, r) # sfs)))
+          (tco_state (TS vs ((v # env, [], r') # (env, op # cd, r) # sfs)))" 
+        using iter_step by fast
+      with Cons Nil show ?thesis by simp
+    next
+      case (Cons op' cd')
+      from evt_lookup have "tco_state (TS (v # TLam env (op' # cd') r' # vs) 
+        ((env, TApply # op # cd, r) # sfs)) \<leadsto>\<^sub>t
+          tco_state (TS vs ((v # env, (op' # cd'), r') # (env, op # cd, r) # sfs))" by simp
+      with CD Cons show ?thesis by (metis iter_one)
+    qed
+  qed
+qed simp_all
+
+lemma iter_tco_eval [simp]: "iter (\<leadsto>\<^sub>t) \<Sigma> \<Sigma>' \<Longrightarrow> jump_free_state \<Sigma> \<Longrightarrow> 
+    iter (\<leadsto>\<^sub>t) (tco_state \<Sigma>) (tco_state \<Sigma>')"
+  by (induction \<Sigma> \<Sigma>' rule: iter.induct) (simp, metis iter_append correcttco jump_free_persists)
 
 end
