05TreeCode/TreeCode.thy
@@ -2,54 +2,63 @@ theory TreeCode
   imports "../00Utils/Environment"
 begin
 
+datatype tree_return =
+    TReturn
+  | TJump
+
 datatype tree_code = 
   TLookup nat
   | TPushCon nat
-  | TPushLam "tree_code list"
+  | TPushLam "tree_code list" tree_return
   | TApply
-  | TReturn
-  | TJump
 
 datatype tclosure = 
   TConst nat
-  | TLam "tclosure list" "tree_code list"
+  | TLam "tclosure list" "tree_code list" tree_return
 
-datatype tree_code_state = TS "tclosure list" "tclosure list list" "tree_code list"
+type_synonym tree_stack_frame = "tclosure list \<times> tree_code list \<times> tree_return"
+
+datatype tree_code_state = TS "tclosure list" "tree_stack_frame list"
 
 inductive evalt :: "tree_code_state \<Rightarrow> tree_code_state \<Rightarrow> bool" (infix "\<leadsto>\<^sub>t" 50) where
   evt_lookup [simp]: "lookup env x = Some v \<Longrightarrow> 
-    TS vs (env # envs) (TLookup x # cd) \<leadsto>\<^sub>t TS (v # vs) (env # envs) cd"
-| evt_pushcon [simp]: "TS vs envs (TPushCon k # cd) \<leadsto>\<^sub>t TS (TConst k # vs) envs cd"
-| evt_pushlam [simp]: "TS vs (env # envs) (TPushLam cd' # cd) \<leadsto>\<^sub>t 
-    TS (TLam env cd' # vs) (env # envs) cd"
-| evt_apply [simp]: "TS (v # TLam env cd' # vs) envs (TApply # cd) \<leadsto>\<^sub>t 
-    TS vs ((v # env) # envs) (cd' @ cd)"
-| evt_return [simp]: "TS vs (env # envs) (TReturn # cd) \<leadsto>\<^sub>t TS vs envs cd"
-| evt_jump [simp]: "TS (v # TLam env' cd' # vs) (env # envs) (TJump # cd) \<leadsto>\<^sub>t 
-    TS vs ((v # env') # envs) (cd' @ cd)"
+    TS vs ((env, TLookup x # cd, r) # sfs) \<leadsto>\<^sub>t TS (v # vs) ((env, cd, r) # sfs)"
+| evt_pushcon [simp]: "TS vs ((env, TPushCon k # cd, r) # sfs) \<leadsto>\<^sub>t 
+    TS (TConst k # vs) ((env, cd, r) # sfs)"
+| evt_pushlam [simp]: "TS vs ((env, TPushLam cd' r' # cd, r) # sfs) \<leadsto>\<^sub>t 
+    TS (TLam env cd' r' # vs) ((env, cd, r) # sfs)"
+| evt_apply [simp]: "TS (v # TLam env cd' r' # vs) ((env, TApply # cd, r) # sfs) \<leadsto>\<^sub>t 
+    TS vs ((v # env, cd', r') # (env, cd, r) # sfs)"
+| evt_return [simp]: "TS vs ((env, [], TReturn) # sfs) \<leadsto>\<^sub>t TS vs sfs"
+| evt_jump [simp]: "TS (v # TLam env' cd' r' # vs) ((env, [], TJump) # sfs) \<leadsto>\<^sub>t 
+    TS vs ((v # env', cd', r') # sfs)"
 
 theorem determinismt: "\<Sigma> \<leadsto>\<^sub>t \<Sigma>' \<Longrightarrow> \<Sigma> \<leadsto>\<^sub>t \<Sigma>'' \<Longrightarrow> \<Sigma>' = \<Sigma>''"
 proof (induction \<Sigma> \<Sigma>' rule: evalt.induct)
-  case (evt_lookup env x v vs envs cd)
+  case (evt_lookup env x v vs cd r sfs)
   from evt_lookup(2, 1) show ?case 
-    by (induction "TS vs (env # envs) (TLookup x # cd)" \<Sigma>'' rule: evalt.induct) simp_all 
+    by (induction "TS vs ((env, TLookup x # cd, r) # sfs)" \<Sigma>'' rule: evalt.induct) simp_all 
 next
-  case (evt_pushcon vs envs k cd)
-  thus ?case by (induction "TS vs envs (TPushCon k # cd)" \<Sigma>'' rule: evalt.induct) simp_all 
-next
-  case (evt_pushlam vs env envs cd' cd)
-  thus ?case by (induction "TS vs (env # envs) (TPushLam cd' # cd)" \<Sigma>'' rule: evalt.induct) simp_all 
-next
-  case (evt_apply v env cd' vs envs cd)
+  case (evt_pushcon vs env k cd r sfs)
   thus ?case 
-    by (induction "TS (v # TLam env cd' # vs) envs (TApply # cd)" \<Sigma>'' rule: evalt.induct) simp_all 
+    by (induction "TS vs ((env, TPushCon k # cd, r) # sfs)" \<Sigma>'' rule: evalt.induct) simp_all 
 next
-  case (evt_return vs env envs cd)
-  thus ?case by (induction "TS vs (env # envs) (TReturn # cd)" \<Sigma>'' rule: evalt.induct) simp_all 
-next
-  case (evt_jump v env' cd' vs env envs cd)
+  case (evt_pushlam vs env cd' r' cd r sfs)
   thus ?case 
-    by (induction "TS (v # TLam env' cd' # vs) (env # envs) (TJump # cd)" \<Sigma>'' rule: evalt.induct) 
+    by (induction "TS vs ((env, TPushLam cd' r' # cd, r) # sfs)" \<Sigma>'' rule: evalt.induct) simp_all 
+next
+  case (evt_apply v env cd' r' vs cd r sfs)
+  thus ?case 
+    by (induction "TS (v # TLam env cd' r' # vs) ((env, TApply # cd, r) # sfs)" \<Sigma>'' 
+        rule: evalt.induct) 
+       simp_all 
+next
+  case (evt_return vs env sfs)
+  thus ?case by (induction "TS vs ((env, [], TReturn) # sfs)" \<Sigma>'' rule: evalt.induct) simp_all 
+next
+  case (evt_jump v env' cd' r' vs env sfs)
+  thus ?case 
+    by (induction "TS (v # TLam env' cd' r' # vs) ((env, [], TJump) # sfs)" \<Sigma>'' rule: evalt.induct) 
        simp_all 
 qed
 
