05TreeCode/TreeCodeConversion.thy
@@ -2,42 +2,38 @@ theory TreeCodeConversion
   imports TreeCode "../04Closure/Closure"
 begin
 
-primrec compile' :: "dexpr \<Rightarrow> tree_code list \<Rightarrow> tree_code list" where
-  "compile' (DVar x) cd = TLookup x # cd"
-| "compile' (DConst k) cd = TPushCon k # cd"
-| "compile' (DLam t e) cd = TPushLam (compile' e [TReturn]) # cd"
-| "compile' (DApp e\<^sub>1 e\<^sub>2) cd = compile' e\<^sub>1 (compile' e\<^sub>2 (TApply # cd))"
+primrec encode' :: "dexpr \<Rightarrow> tree_code list \<Rightarrow> tree_code list" where
+  "encode' (DVar x) cd = TLookup x # cd"
+| "encode' (DConst k) cd = TPushCon k # cd"
+| "encode' (DLam t e) cd = TPushLam (encode' e []) TReturn # cd"
+| "encode' (DApp e\<^sub>1 e\<^sub>2) cd = encode' e\<^sub>1 (encode' e\<^sub>2 (TApply # cd))"
 
-definition compile :: "dexpr \<Rightarrow> tree_code list" where
-  "compile e = compile' e [TReturn]"
+definition encode :: "dexpr \<Rightarrow> tree_code list" where
+  "encode e = encode' e []"
 
-primrec compile_closure :: "closure \<Rightarrow> tclosure" where
-  "compile_closure (CConst k) = TConst k"
-| "compile_closure (CLam t cs e) = TLam (map compile_closure cs) (compile e)"
+primrec encode_closure :: "closure \<Rightarrow> tclosure" where
+  "encode_closure (CConst k) = TConst k"
+| "encode_closure (CLam t cs e) = TLam (map encode_closure cs) (encode e) TReturn"
 
 fun vals_from_stack :: "cframe list \<Rightarrow> tclosure list" where
   "vals_from_stack [] = []"
 | "vals_from_stack (CApp1 cs e # s) = vals_from_stack s"
-| "vals_from_stack (CApp2 c # s) = compile_closure c # vals_from_stack s"
+| "vals_from_stack (CApp2 c # s) = encode_closure c # vals_from_stack s"
 | "vals_from_stack (CReturn cs # s) = vals_from_stack s"
 
-fun envs_from_stack :: "cframe list \<Rightarrow> tclosure list list" where
-  "envs_from_stack [] = []"
-| "envs_from_stack (CApp1 cs e # s) = envs_from_stack s"
-| "envs_from_stack (CApp2 c # s) = envs_from_stack s"
-| "envs_from_stack (CReturn cs # s) = map compile_closure cs # envs_from_stack s"
+fun stack_from_stack :: "cframe list \<Rightarrow> (tclosure list \<times> tree_code list \<times> tree_return) list" where
+  "stack_from_stack [] = [([], [], TReturn)]"
+| "stack_from_stack (CApp1 cs e # s) = (case hd (stack_from_stack s) of 
+    (env, cd, r) \<Rightarrow> (env, encode' e (TApply # cd), r) # tl (stack_from_stack s))"
+| "stack_from_stack (CApp2 c # s) = (case hd (stack_from_stack s) of 
+    (env, cd, r) \<Rightarrow> (env, TApply # cd, r) # tl (stack_from_stack s))"
+| "stack_from_stack (CReturn cs # s) = (map encode_closure cs, [], TReturn) # stack_from_stack s"
 
-fun code_from_stack :: "cframe list \<Rightarrow> tree_code list" where
-  "code_from_stack [] = []"
-| "code_from_stack (CApp1 cs e # s) = compile' e (TApply # code_from_stack s)"
-| "code_from_stack (CApp2 c # s) = TApply # code_from_stack s"
-| "code_from_stack (CReturn cs # s) = TReturn # code_from_stack s"
-
-primrec compile_state :: "closure_state \<Rightarrow> tree_code_state" where
-  "compile_state (CSE s cs e) = 
-    TS (vals_from_stack s) (envs_from_stack s) (compile' e (code_from_stack s))"
-| "compile_state (CSC s c) = 
-    TS (compile_closure c # vals_from_stack s) (envs_from_stack s) (code_from_stack s)"
+primrec encode_state :: "closure_state \<Rightarrow> tree_code_state" where
+  "encode_state (CSE s cs e) = (case hd (stack_from_stack s) of 
+    (env, cd, r) \<Rightarrow> TS (vals_from_stack s) ((env, encode' e cd, r) # tl (stack_from_stack s)))"
+| "encode_state (CSC s c) = 
+    TS (encode_closure c # vals_from_stack s) (stack_from_stack s)"
 
 primrec unzip :: "dexpr \<Rightarrow> dexpr \<times> dexpr list" where
   "unzip (DVar x) = (DVar x, [])"
@@ -45,52 +41,44 @@ primrec unzip :: "dexpr \<Rightarrow> dexpr \<times> dexpr list" where
 | "unzip (DLam t e) = (DLam t e, [])"
 | "unzip (DApp e\<^sub>1 e\<^sub>2) = (case unzip e\<^sub>1 of (e, es) \<Rightarrow> (e, e\<^sub>2 # es))"
 
-primrec zipcompile :: "dexpr list \<Rightarrow> tree_code list \<Rightarrow> tree_code list" where 
-  "zipcompile [] acc = acc"
-| "zipcompile (e # es) acc = zipcompile es (compile' e (TApply # acc))"
+primrec zip_encode :: "dexpr list \<Rightarrow> tree_code list \<Rightarrow> tree_code list" where 
+  "zip_encode [] acc = acc"
+| "zip_encode (e # es) acc = zip_encode es (encode' e (TApply # acc))"
 
-lemma [simp]: "compile' e cd @ cd' = compile' e (cd @ cd')"
+lemma [simp]: "encode' e cd @ cd' = encode' e (cd @ cd')"
   by (induction e arbitrary: cd) simp_all
 
-lemma [simp]: "unzip e = (e', es) \<Longrightarrow> compile' e' (zipcompile es acc) = compile' e acc"
+lemma [simp]: "unzip e = (e', es) \<Longrightarrow> encode' e' (zip_encode es acc) = encode' e acc"
   by (induction e arbitrary: e' es acc) (auto split: prod.splits)
 
 lemma [simp]: "vals_from_stack (map (CApp1 cs) (rev es) @ s) = vals_from_stack s"
   by (induction es arbitrary: s) simp_all
 
-lemma [simp]: "envs_from_stack (map (CApp1 cs) (rev es) @ s) = envs_from_stack s"
-  by (induction es arbitrary: s) simp_all
+lemma [simp]: "stack_from_stack s = (env, cd, r) # sfs \<Longrightarrow> 
+    stack_from_stack (map (CApp1 cs) (rev es) @ s) = (env, zip_encode es cd, r) # sfs"
+  by (induction es arbitrary: s cd) simp_all
 
-lemma [simp]: "code_from_stack (map (CApp1 cs) (rev es) @ s) = zipcompile es (code_from_stack s)"
-  by (induction es arbitrary: s) simp_all
-
-lemma [dest]: "compile' e cd' = TLookup x # cd \<Longrightarrow> 
-    (\<And>es. unzip e = (DVar x, es) \<Longrightarrow> cd = zipcompile es cd' \<Longrightarrow> P) \<Longrightarrow> P"
+lemma [dest]: "encode' e cd' = TLookup x # cd \<Longrightarrow> 
+    (\<And>es. unzip e = (DVar x, es) \<Longrightarrow> cd = zip_encode es cd' \<Longrightarrow> P) \<Longrightarrow> P"
   by (induction e arbitrary: cd') fastforce+
 
-lemma [dest]: "compile' e cd' = TPushCon k # cd \<Longrightarrow> 
-    (\<And>es. unzip e = (DConst k, es) \<Longrightarrow> cd = zipcompile es cd' \<Longrightarrow> P) \<Longrightarrow> P"
+lemma [dest]: "encode' e cd' = TPushCon k # cd \<Longrightarrow> 
+    (\<And>es. unzip e = (DConst k, es) \<Longrightarrow> cd = zip_encode es cd' \<Longrightarrow> P) \<Longrightarrow> P"
   by (induction e arbitrary: cd') fastforce+
 
-lemma compile_to_pushlam' [dest]: "compile' e cd' = TPushLam cd'' # cd \<Longrightarrow> 
-  (\<And>es t e'. unzip e = (DLam t e', es) \<Longrightarrow> cd'' = compile e' \<Longrightarrow> 
-    cd = zipcompile es cd' \<Longrightarrow> P) \<Longrightarrow> P"
-  using compile_def by (induction e arbitrary: cd') fastforce+
+lemma encode_to_pushlam' [dest]: "encode' e cd' = TPushLam cd'' r # cd \<Longrightarrow> 
+  (\<And>es t e'. unzip e = (DLam t e', es) \<Longrightarrow> cd'' = encode e' \<Longrightarrow> r = TReturn \<Longrightarrow> 
+    cd = zip_encode es cd' \<Longrightarrow> P) \<Longrightarrow> P"
+  using encode_def by (induction e arbitrary: cd') fastforce+
 
-lemma [dest]: "compile' e cd' = TApply # cd \<Longrightarrow> P"
+lemma [dest]: "encode' e cd' = TApply # cd \<Longrightarrow> P"
   by (induction e arbitrary: cd') simp_all
 
-lemma [dest]: "compile' e cd' = TReturn # cd \<Longrightarrow> P"
-  by (induction e arbitrary: cd') simp_all
-
-lemma [dest]: "compile' e cd' = TJump # cd \<Longrightarrow> P"
-  by (induction e arbitrary: cd') simp_all
-
-lemma [dest]: "compile_closure c = TConst k \<Longrightarrow> c = CConst k"
+lemma [dest]: "encode_closure c = TConst k \<Longrightarrow> c = CConst k"
   by (induction c) simp_all
 
-lemma compile_lam_closure [dest]: "compile_closure c = TLam env cd \<Longrightarrow> (\<And>t cs e. 
-    c = CLam t cs e \<Longrightarrow> env = map compile_closure cs \<Longrightarrow> cd = compile e \<Longrightarrow> P) \<Longrightarrow> P"
+lemma encode_lam_closure [dest]: "encode_closure c = TLam env cd r \<Longrightarrow> (\<And>t cs e. 
+    c = CLam t cs e \<Longrightarrow> env = map encode_closure cs \<Longrightarrow> cd = encode e \<Longrightarrow> r = TReturn \<Longrightarrow> P) \<Longrightarrow> P"
   by (induction c) simp_all
 
 lemma tc_latest_environment [simp]: "s @ CApp1 cs e # s' :\<^sub>c t \<rightarrow> t' \<Longrightarrow> 
@@ -102,86 +90,102 @@ proof (induction s arbitrary: t)
   ultimately show ?case by simp
 qed fastforce+
 
-lemma compile_stack_to_lookup [dest]: "code_from_stack s = TLookup x # cd \<Longrightarrow> 
-  \<exists>cs e es s'. s = CApp1 cs e # s' \<and> unzip e = (DVar x, es) \<and> 
-    cd = zipcompile es (TApply # code_from_stack s')"
-  by (induction s rule: code_from_stack.induct) auto
+lemma [simp]: "stack_from_stack s \<noteq> []"
+  by (induction s rule: stack_from_stack.induct) (simp_all split: prod.splits)
 
-lemma compile_stack_to_pushcon [dest]: "code_from_stack s = TPushCon k # cd \<Longrightarrow> 
+lemma [simp]: "\<exists>env cd r. hd (stack_from_stack s) = (env, cd, r)"
+  by (induction s rule: stack_from_stack.induct) (simp_all split: prod.splits)
+
+lemma encode_stack_to_lookup [dest]: "stack_from_stack s = (env, TLookup x # cd, r) # sfs \<Longrightarrow> 
+  \<exists>cs e es s' cd'. s = CApp1 cs e # s' \<and> stack_from_stack s' = (env, cd', r) # sfs \<and> 
+    unzip e = (DVar x, es) \<and> cd = zip_encode es (TApply # cd')"
+proof (induction s rule: stack_from_stack.induct)
+  case (2 cs e s)
+  obtain env' cd' r' where "hd (stack_from_stack s) = (env', cd', r')" by fastforce
+  moreover with 2 have E: "env' = env \<and> r' = r \<and> encode' e (TApply # cd') = TLookup x # cd \<and> 
+    sfs = tl (stack_from_stack s)" by simp
+  ultimately have "stack_from_stack s = (env, cd', r) # sfs" 
+    by (cases "stack_from_stack s") simp_all
+  moreover from E obtain es where "unzip e = (DVar x, es) \<and> cd = zip_encode es (TApply # cd')"
+    by blast
+  ultimately show ?case by fastforce
+qed (simp_all split: prod.splits)
+
+lemma encode_stack_to_pushcon [dest]: "code_from_stack s = TPushCon k # cd \<Longrightarrow> 
   \<exists>cs e es s'. s = CApp1 cs e # s' \<and> unzip e = (DConst k, es) \<and>
-    cd = zipcompile es (TApply # code_from_stack s')"
+    cd = zip_encode es (TApply # code_from_stack s')"
   by (induction s rule: code_from_stack.induct) auto
 
-lemma compile_stack_to_pushlam [dest]: "code_from_stack s = TPushLam cd' # cd \<Longrightarrow> 
+lemma encode_stack_to_pushlam [dest]: "code_from_stack s = TPushLam cd' # cd \<Longrightarrow> 
   \<exists>cs e es s' t e'. s = CApp1 cs e # s' \<and> unzip e = (DLam t e', es) \<and>
-    cd = zipcompile es (TApply # code_from_stack s') \<and> cd' = compile e'"
+    cd = zip_encode es (TApply # code_from_stack s') \<and> cd' = encode e'"
 proof (induction s rule: code_from_stack.induct)
   case (2 cs e s)
-  hence "compile' e (TApply # code_from_stack s) = TPushLam cd' # cd" by auto
-  moreover then obtain es t e' where "unzip e = (DLam t e', es) \<and> cd' = compile e' \<and> 
-    cd = zipcompile es (TApply # code_from_stack s)" by blast
+  hence "encode' e (TApply # code_from_stack s) = TPushLam cd' # cd" by auto
+  moreover then obtain es t e' where "unzip e = (DLam t e', es) \<and> cd' = encode e' \<and> 
+    cd = zip_encode es (TApply # code_from_stack s)" by blast
   ultimately show ?case by simp
 qed simp_all
 
-lemma compile_stack_to_apply [dest]: "code_from_stack s = TApply # cd \<Longrightarrow> 
+lemma encode_stack_to_apply [dest]: "code_from_stack s = TApply # cd \<Longrightarrow> 
     \<exists>s' c. s = CApp2 c # s' \<and> cd = code_from_stack s'"
   by (induction s rule: code_from_stack.induct) auto
 
-lemma compile_stack_to_return [dest]: "code_from_stack s = TReturn # cd \<Longrightarrow> 
+lemma encode_stack_to_return [dest]: "code_from_stack s = TReturn # cd \<Longrightarrow> 
     \<exists>cs s'. s = CReturn cs # s' \<and> cd = code_from_stack s'"
   by (induction s rule: code_from_stack.induct) auto
  
-lemma compile_stack_to_jump [dest]: "code_from_stack s = TJump # cd \<Longrightarrow> False"
+lemma encode_stack_to_jump [dest]: "code_from_stack s = TJump # cd \<Longrightarrow> False"
   by (induction s rule: code_from_stack.induct) auto
 
-lemma compile_to_lookup [simp]: "\<Sigma> :\<^sub>c t \<Longrightarrow> compile_state \<Sigma> = TS vs envs (TLookup x # cd) \<Longrightarrow> 
-  (\<exists>s cs e es. \<Sigma> = CSE s cs e \<and> unzip e = (DVar x, es) \<and> cd = zipcompile es (code_from_stack s) \<and>
+lemma encode_to_lookup [simp]: "\<Sigma> :\<^sub>c t \<Longrightarrow> encode_state \<Sigma> = TS vs envs (TLookup x # cd) \<Longrightarrow> 
+  (\<exists>s cs e es. \<Sigma> = CSE s cs e \<and> unzip e = (DVar x, es) \<and> cd = zip_encode es (code_from_stack s) \<and>
     vs = vals_from_stack s \<and> envs = envs_from_stack s) \<or> (\<exists>s c cs e es. 
       \<Sigma> = CSC (CApp1 cs e # s) c \<and> unzip e = (DVar x, es) \<and> envs = envs_from_stack s \<and>
-        cd = zipcompile es (TApply # code_from_stack s) \<and> 
-          vs = compile_closure c # vals_from_stack s)"
+        cd = zip_encode es (TApply # code_from_stack s) \<and> 
+          vs = encode_closure c # vals_from_stack s)"
   by (induction \<Sigma> t rule: typecheck_closure_state.induct) auto
 
-lemma compile_to_pushcon [simp]: "\<Sigma> :\<^sub>c t \<Longrightarrow> compile_state \<Sigma> = TS vs envs (TPushCon k # cd) \<Longrightarrow> 
-  (\<exists>s cs e es. \<Sigma> = CSE s cs e \<and> unzip e = (DConst k, es) \<and> cd = zipcompile es (code_from_stack s) \<and>
+lemma encode_to_pushcon [simp]: "\<Sigma> :\<^sub>c t \<Longrightarrow> encode_state \<Sigma> = TS vs envs (TPushCon k # cd) \<Longrightarrow> 
+  (\<exists>s cs e es. \<Sigma> = CSE s cs e \<and> unzip e = (DConst k, es) \<and> cd = zip_encode es (code_from_stack s) \<and>
     vs = vals_from_stack s \<and> envs = envs_from_stack s) \<or> (\<exists>s c cs e es. 
       \<Sigma> = CSC (CApp1 cs e # s) c \<and> unzip e = (DConst k, es) \<and> envs = envs_from_stack s \<and>
-        cd = zipcompile es (TApply # code_from_stack s) \<and> 
-          vs = compile_closure c # vals_from_stack s)"
+        cd = zip_encode es (TApply # code_from_stack s) \<and> 
+          vs = encode_closure c # vals_from_stack s)"
   by (induction \<Sigma> t rule: typecheck_closure_state.induct) auto
 
-lemma compile_to_pushlam [simp]: "\<Sigma> :\<^sub>c t \<Longrightarrow> compile_state \<Sigma> = TS vs envs (TPushLam cd' # cd) \<Longrightarrow> 
+lemma encode_to_pushlam [simp]: "\<Sigma> :\<^sub>c t \<Longrightarrow> encode_state \<Sigma> = TS vs envs (TPushLam cd' # cd) \<Longrightarrow> 
   (\<exists>s cs e es tt e'. \<Sigma> = CSE s cs e \<and> unzip e = (DLam tt e', es) \<and> 
-    cd = zipcompile es (code_from_stack s) \<and> cd' = compile e' \<and> vs = vals_from_stack s \<and> 
+    cd = zip_encode es (code_from_stack s) \<and> cd' = encode e' \<and> vs = vals_from_stack s \<and> 
       envs = envs_from_stack s) \<or> (\<exists>s c cs e es tt e'. \<Sigma> = CSC (CApp1 cs e # s) c \<and> 
-        unzip e = (DLam tt e', es) \<and> cd = zipcompile es (TApply # code_from_stack s) \<and> 
-          cd' = compile e' \<and> vs = compile_closure c # vals_from_stack s \<and> 
+        unzip e = (DLam tt e', es) \<and> cd = zip_encode es (TApply # code_from_stack s) \<and> 
+          cd' = encode e' \<and> vs = encode_closure c # vals_from_stack s \<and> 
             envs = envs_from_stack s)"
 proof (induction \<Sigma> t rule: typecheck_closure_state.induct)
   case (tcc_state_ev s t' t cs ts e)
-  hence "compile' e (code_from_stack s) = TPushLam cd' # cd" by simp
-  then obtain es tt e' where "unzip e = (DLam tt e', es) \<and> cd' = compile e'  \<and> 
-    cd = zipcompile es (code_from_stack s)" by (metis compile_to_pushlam')
+  hence "encode' e (code_from_stack s) = TPushLam cd' # cd" by simp
+  then obtain es tt e' where "unzip e = (DLam tt e', es) \<and> cd' = encode e'  \<and> 
+    cd = zip_encode es (code_from_stack s)" by (metis encode_to_pushlam')
   with tcc_state_ev show ?case by fastforce
 next
   case (tcc_state_ret s t' t c)
   moreover then obtain cs e es s' tt e' where "s = CApp1 cs e # s' \<and> unzip e = (DLam tt e', es) \<and>
-    cd = zipcompile es (TApply # code_from_stack s') \<and> cd' = compile e'" 
-      using compile_stack_to_pushlam by auto
+    cd = zip_encode es (TApply # code_from_stack s') \<and> cd' = encode e'" 
+      using encode_stack_to_pushlam by auto
   ultimately show ?case by fastforce
 qed
 
-lemma compile_to_apply [simp]: "\<Sigma> :\<^sub>c t \<Longrightarrow> compile_state \<Sigma> = TS vs envs (TApply # cd) \<Longrightarrow> 
+lemma encode_to_apply [simp]: "\<Sigma> :\<^sub>c t \<Longrightarrow> encode_state \<Sigma> = TS vs envs (TApply # cd) \<Longrightarrow> 
   \<exists>s c c'. \<Sigma> = CSC (CApp2 c' # s) c \<and> cd = code_from_stack s \<and> envs = envs_from_stack s \<and> 
-    vs = compile_closure c # compile_closure c' # vals_from_stack s"
+    vs = encode_closure c # encode_closure c' # vals_from_stack s"
   by (induction \<Sigma> t rule: typecheck_closure_state.induct) auto
 
-lemma compile_to_return [simp]: "\<Sigma> :\<^sub>c t \<Longrightarrow> compile_state \<Sigma> = TS vs envs (TReturn # cd) \<Longrightarrow> 
+lemma encode_to_return [simp]: "\<Sigma> :\<^sub>c t \<Longrightarrow> encode_state \<Sigma> = TS vs envs (TReturn # cd) \<Longrightarrow> 
   \<exists>cs s c. \<Sigma> = CSC (CReturn cs # s) c \<and> cd = code_from_stack s \<and> 
-    envs = map compile_closure cs # envs_from_stack s \<and> vs = compile_closure c # vals_from_stack s"
+    envs = map encode_closure cs # envs_from_stack s \<and> vs = encode_closure c # vals_from_stack s"
   by (induction \<Sigma> t rule: typecheck_closure_state.induct) auto
 
-lemma compile_to_jump [simp]: "\<Sigma> :\<^sub>c t \<Longrightarrow> compile_state \<Sigma> = TS vs envs (TJump # cd) \<Longrightarrow> False"
+lemma encode_to_jump [simp]: "\<Sigma> :\<^sub>c t \<Longrightarrow> encode_state \<Sigma> = TS vs envs (TJump # cd) \<Longrightarrow> False"
   by (induction \<Sigma> t rule: typecheck_closure_state.induct) (auto split: tree_code_state.splits)
 
 lemma [simp]: "unzip e = (e', es) \<Longrightarrow> 
@@ -196,37 +200,37 @@ proof (induction e arbitrary: s es)
 qed simp_all 
 
 lemma [simp]: "env # envs = envs_from_stack s \<Longrightarrow> latest_environment s = Some cs \<Longrightarrow> 
-    env = map compile_closure cs"
+    env = map encode_closure cs"
   by (induction s rule: latest_environment.induct) simp_all
 
-theorem correctt [simp]: "compile_state \<Sigma>\<^sub>c \<leadsto>\<^sub>t \<Sigma>\<^sub>t' \<Longrightarrow> \<Sigma>\<^sub>c :\<^sub>c t \<Longrightarrow>
-  \<exists>\<Sigma>\<^sub>c'. iter (\<leadsto>\<^sub>c) \<Sigma>\<^sub>c \<Sigma>\<^sub>c' \<and> \<Sigma>\<^sub>t' = compile_state \<Sigma>\<^sub>c'"
-proof (induction "compile_state \<Sigma>\<^sub>c" \<Sigma>\<^sub>t' rule: evalt.induct)
+theorem correctt [simp]: "encode_state \<Sigma>\<^sub>c \<leadsto>\<^sub>t \<Sigma>\<^sub>t' \<Longrightarrow> \<Sigma>\<^sub>c :\<^sub>c t \<Longrightarrow>
+  \<exists>\<Sigma>\<^sub>c'. iter (\<leadsto>\<^sub>c) \<Sigma>\<^sub>c \<Sigma>\<^sub>c' \<and> \<Sigma>\<^sub>t' = encode_state \<Sigma>\<^sub>c'"
+proof (induction "encode_state \<Sigma>\<^sub>c" \<Sigma>\<^sub>t' rule: evalt.induct)
   case (evt_lookup env x v vs envs cd)
   moreover hence "(\<exists>s cs e es. \<Sigma>\<^sub>c = CSE s cs e \<and> unzip e = (DVar x, es) \<and> 
-    cd = zipcompile es (code_from_stack s) \<and> vs = vals_from_stack s \<and> 
+    cd = zip_encode es (code_from_stack s) \<and> vs = vals_from_stack s \<and> 
       env # envs = envs_from_stack s) \<or> (\<exists>s c cs e es. \<Sigma>\<^sub>c = CSC (CApp1 cs e # s) c \<and> 
         unzip e = (DVar x, es) \<and> env # envs = envs_from_stack s \<and> 
-          cd = zipcompile es (TApply # code_from_stack s) \<and> 
-            vs = compile_closure c # vals_from_stack s)" using compile_to_lookup by simp
+          cd = zip_encode es (TApply # code_from_stack s) \<and> 
+            vs = encode_closure c # vals_from_stack s)" using encode_to_lookup by simp
   ultimately show ?case
   proof (induction \<Sigma>\<^sub>c)
     case (CSE s cs e)
-    then obtain es where E: "unzip e = (DVar x, es) \<and> cd = zipcompile es (code_from_stack s) \<and>
+    then obtain es where E: "unzip e = (DVar x, es) \<and> cd = zip_encode es (code_from_stack s) \<and>
       vs = vals_from_stack s \<and> env # envs = envs_from_stack s" by auto 
     hence X: "iter (\<leadsto>\<^sub>c) (CSE s cs e) (CSE (map (CApp1 cs) (rev es) @ s) cs (DVar x))" by simp
     from CSE obtain t' ts where "(s :\<^sub>c t' \<rightarrow> t) \<and> (cs :\<^sub>c\<^sub>l\<^sub>s ts) \<and>
       latest_environment s = Some cs \<and> (ts \<turnstile>\<^sub>d e : t')" by fastforce
-    with E have "env = map compile_closure cs" by fastforce
-    with CSE obtain c where C: "lookup cs x = Some c \<and> compile_closure c = v" by fastforce
+    with E have "env = map encode_closure cs" by fastforce
+    with CSE obtain c where C: "lookup cs x = Some c \<and> encode_closure c = v" by fastforce
     with X have "iter (\<leadsto>\<^sub>c) (CSE s cs e) (CSC (map (CApp1 cs) (rev es) @ s) c)" by simp
     with E C show ?case by fastforce
   next
     case (CSC s c)
     then obtain s' cs e es where S: "s = CApp1 cs e # s' \<and> 
       unzip e = (DVar x, es) \<and> env # envs = envs_from_stack s' \<and> 
-        cd = zipcompile es (TApply # code_from_stack s') \<and> 
-          vs = compile_closure c # vals_from_stack s'" by auto
+        cd = zip_encode es (TApply # code_from_stack s') \<and> 
+          vs = encode_closure c # vals_from_stack s'" by auto
     hence "iter (\<leadsto>\<^sub>c) (CSE (CApp2 c # s') cs e) 
       (CSE (map (CApp1 cs) (rev es) @ CApp2 c # s') cs (DVar x))" by simp
     moreover have "CSC (CApp1 cs e # s') c \<leadsto>\<^sub>c CSE (CApp2 c # s') cs e" by simp
@@ -235,8 +239,8 @@ proof (induction "compile_state \<Sigma>\<^sub>c" \<Sigma>\<^sub>t' rule: evalt.
     from CSC obtain t' where "(s :\<^sub>c t' \<rightarrow> t) \<and> (c :\<^sub>c\<^sub>l t')" by fastforce
     with S obtain ts t\<^sub>1 t\<^sub>2 where "t' = Arrow t\<^sub>1 t\<^sub>2 \<and> (cs :\<^sub>c\<^sub>l\<^sub>s ts) \<and> (ts \<turnstile>\<^sub>d e : t\<^sub>1) \<and> (s' :\<^sub>c t\<^sub>2 \<rightarrow> t) \<and> 
       latest_environment s' = Some cs" by fastforce
-    with S have "env = map compile_closure cs" by fastforce
-    with CSC obtain c' where C: "lookup cs x = Some c' \<and> compile_closure c' = v" by fastforce
+    with S have "env = map encode_closure cs" by fastforce
+    with CSC obtain c' where C: "lookup cs x = Some c' \<and> encode_closure c' = v" by fastforce
     with X have "iter (\<leadsto>\<^sub>c) (CSC (CApp1 cs e # s') c) 
       (CSC (map (CApp1 cs) (rev es) @ CApp2 c # s') c')" by simp
     with S C show ?case by fastforce
@@ -244,14 +248,14 @@ proof (induction "compile_state \<Sigma>\<^sub>c" \<Sigma>\<^sub>t' rule: evalt.
 next
   case (evt_pushcon vs envs k cd)
   hence "(\<exists>s cs e es. \<Sigma>\<^sub>c = CSE s cs e \<and> unzip e = (DConst k, es) \<and> 
-    cd = zipcompile es (code_from_stack s) \<and> vs = vals_from_stack s \<and> envs = envs_from_stack s) \<or> 
+    cd = zip_encode es (code_from_stack s) \<and> vs = vals_from_stack s \<and> envs = envs_from_stack s) \<or> 
       (\<exists>s c cs e es. \<Sigma>\<^sub>c = CSC (CApp1 cs e # s) c \<and> unzip e = (DConst k, es) \<and> 
-        envs = envs_from_stack s \<and> cd = zipcompile es (TApply # code_from_stack s) \<and> 
-          vs = compile_closure c # vals_from_stack s)" using compile_to_pushcon by simp
+        envs = envs_from_stack s \<and> cd = zip_encode es (TApply # code_from_stack s) \<and> 
+          vs = encode_closure c # vals_from_stack s)" using encode_to_pushcon by simp
   thus ?case
   proof (induction \<Sigma>\<^sub>c)
     case (CSE s cs e)
-    then obtain es where E: "unzip e = (DConst k, es) \<and> cd = zipcompile es (code_from_stack s) \<and> 
+    then obtain es where E: "unzip e = (DConst k, es) \<and> cd = zip_encode es (code_from_stack s) \<and> 
       vs = vals_from_stack s \<and> envs = envs_from_stack s" by auto
     hence "iter (\<leadsto>\<^sub>c) (CSE s cs e) (CSE (map (CApp1 cs) (rev es) @ s) cs (DConst k))" by simp
     moreover have "CSE (map (CApp1 cs) (rev es) @ s) cs (DConst k) \<leadsto>\<^sub>c 
@@ -261,8 +265,8 @@ next
   next
     case (CSC s c)
     then obtain s' cs e es where S: "s = CApp1 cs e # s' \<and> unzip e = (DConst k, es) \<and> 
-        envs = envs_from_stack s' \<and> cd = zipcompile es (TApply # code_from_stack s') \<and> 
-          vs = compile_closure c # vals_from_stack s'" by auto
+        envs = envs_from_stack s' \<and> cd = zip_encode es (TApply # code_from_stack s') \<and> 
+          vs = encode_closure c # vals_from_stack s'" by auto
     hence "iter (\<leadsto>\<^sub>c) (CSE (CApp2 c # s') cs e) 
       (CSE (map (CApp1 cs) (rev es) @ CApp2 c # s') cs (DConst k))" by simp
     moreover have "CSC (CApp1 cs e # s') c \<leadsto>\<^sub>c CSE (CApp2 c # s') cs e" by simp
@@ -278,10 +282,10 @@ next
   thus ?case
   proof (induction \<Sigma>\<^sub>c)
     case (CSE s cs e)
-    moreover hence "compile_state (CSE s cs e) = TS vs (env # envs) (TPushLam cd' # cd)" by simp
+    moreover hence "encode_state (CSE s cs e) = TS vs (env # envs) (TPushLam cd' # cd)" by simp
     ultimately obtain es tt e' where E: "unzip e = (DLam tt e', es) \<and> 
-      cd = zipcompile es (code_from_stack s) \<and> cd' = compile e' \<and> 
-        vs = vals_from_stack s \<and> env # envs = envs_from_stack s" using compile_to_pushlam by blast
+      cd = zip_encode es (code_from_stack s) \<and> cd' = encode e' \<and> 
+        vs = vals_from_stack s \<and> env # envs = envs_from_stack s" using encode_to_pushlam by blast
     hence "iter (\<leadsto>\<^sub>c) (CSE s cs e) (CSE (map (CApp1 cs) (rev es) @ s) cs (DLam tt e'))" by simp
     moreover have "CSE (map (CApp1 cs) (rev es) @ s) cs (DLam tt e') \<leadsto>\<^sub>c 
       CSC (map (CApp1 cs) (rev es) @ s) (CLam tt cs e')" by simp
@@ -290,11 +294,11 @@ next
     with CSE E show ?case by fastforce
   next
     case (CSC s c)
-    moreover hence "compile_state (CSC s c) = TS vs (env # envs) (TPushLam cd' # cd)" by simp
+    moreover hence "encode_state (CSC s c) = TS vs (env # envs) (TPushLam cd' # cd)" by simp
     ultimately obtain s' cs e es tt e' where S: "s = CApp1 cs e # s' \<and> unzip e = (DLam tt e', es) \<and> 
-      cd = zipcompile es (TApply # code_from_stack s') \<and> cd' = compile e' \<and> 
-        vs = compile_closure c # vals_from_stack s' \<and> env # envs = envs_from_stack s'" 
-      using compile_to_pushlam by blast
+      cd = zip_encode es (TApply # code_from_stack s') \<and> cd' = encode e' \<and> 
+        vs = encode_closure c # vals_from_stack s' \<and> env # envs = envs_from_stack s'" 
+      using encode_to_pushlam by blast
     hence "iter (\<leadsto>\<^sub>c) (CSE (CApp2 c # s') cs e) 
       (CSE (map (CApp1 cs) (rev es) @ CApp2 c # s') cs (DLam tt e'))" by simp
     moreover have "CSC (CApp1 cs e # s') c \<leadsto>\<^sub>c CSE (CApp2 c # s') cs e" by simp
@@ -310,59 +314,59 @@ next
   thus ?case
   proof (induction \<Sigma>\<^sub>c)
     case (CSE s cs e)
-    moreover hence "compile_state (CSE s cs e) = TS (v # TLam env cd' # vs) envs (TApply # cd)"
+    moreover hence "encode_state (CSE s cs e) = TS (v # TLam env cd' # vs) envs (TApply # cd)"
       by simp
-    ultimately show ?case using compile_to_apply by blast
+    ultimately show ?case using encode_to_apply by blast
   next
     case (CSC s c)
-    moreover hence "compile_state (CSC s c) = TS (v # TLam env cd' # vs) envs (TApply # cd)" by simp
+    moreover hence "encode_state (CSC s c) = TS (v # TLam env cd' # vs) envs (TApply # cd)" by simp
     ultimately obtain s' c' where S: "s = CApp2 c' # s' \<and> cd = code_from_stack s' \<and> 
-      envs = envs_from_stack s' \<and> v = compile_closure c \<and> TLam env cd' = compile_closure c' \<and> 
-        vs = vals_from_stack s'" using compile_to_apply by blast
-    then obtain t cs e where C: "c' = CLam t cs e \<and> env = map compile_closure cs \<and> cd' = compile e" 
-      by (metis compile_lam_closure)
+      envs = envs_from_stack s' \<and> v = encode_closure c \<and> TLam env cd' = encode_closure c' \<and> 
+        vs = vals_from_stack s'" using encode_to_apply by blast
+    then obtain t cs e where C: "c' = CLam t cs e \<and> env = map encode_closure cs \<and> cd' = encode e" 
+      by (metis encode_lam_closure)
     have "CSC (CApp2 (CLam t cs e) # s') c \<leadsto>\<^sub>c CSE (CReturn (c # cs) # s') (c # cs) e" by simp
     hence "iter (\<leadsto>\<^sub>c) (CSC (CApp2 (CLam t cs e) # s') c) (CSE (CReturn (c # cs) # s') (c # cs) e)" 
       by (metis iter_step iter_refl)
-    with S C show ?case using compile_def by fastforce
+    with S C show ?case using encode_def by fastforce
   qed
 next
   case (evt_return vs env envs cd)
   thus ?case
   proof (induction \<Sigma>\<^sub>c)
     case (CSE s cs e)
-    moreover hence "compile_state (CSE s cs e) = TS vs (env # envs) (TReturn # cd)" by simp
-    ultimately show ?case using compile_to_return by blast
+    moreover hence "encode_state (CSE s cs e) = TS vs (env # envs) (TReturn # cd)" by simp
+    ultimately show ?case using encode_to_return by blast
   next
     case (CSC s c)
-    moreover hence "compile_state (CSC s c) = TS vs (env # envs) (TReturn # cd)" by simp
+    moreover hence "encode_state (CSC s c) = TS vs (env # envs) (TReturn # cd)" by simp
     ultimately obtain cs s' where S: "s = CReturn cs # s' \<and> cd = code_from_stack s' \<and> 
-      env = map compile_closure cs \<and> envs = envs_from_stack s' \<and> 
-        vs = compile_closure c # vals_from_stack s'" using compile_to_return by blast
+      env = map encode_closure cs \<and> envs = envs_from_stack s' \<and> 
+        vs = encode_closure c # vals_from_stack s'" using encode_to_return by blast
     have "CSC (CReturn cs # s') c \<leadsto>\<^sub>c CSC s' c" by simp
     hence "iter (\<leadsto>\<^sub>c) (CSC (CReturn cs # s') c) (CSC s' c)" by (metis iter_step iter_refl)
     with S show ?case by fastforce
   qed
 next
   case (evt_jump v env' cd' vs env envs cd)
-  thus ?case by (metis compile_to_jump)
+  thus ?case by (metis encode_to_jump)
 qed
 
 lemma lookup_latest [simp]: "latest_environment s = Some cs \<Longrightarrow> 
-    \<exists>envs. envs_from_stack s = map compile_closure cs # envs"
+    \<exists>envs. envs_from_stack s = map encode_closure cs # envs"
   by (induction s rule: envs_from_stack.induct) simp_all
 
-theorem completet [simp]: "\<Sigma> \<leadsto>\<^sub>c \<Sigma>' \<Longrightarrow> \<Sigma> :\<^sub>c t \<Longrightarrow> iter (\<leadsto>\<^sub>t) (compile_state \<Sigma>) (compile_state \<Sigma>')"
+theorem completet [simp]: "\<Sigma> \<leadsto>\<^sub>c \<Sigma>' \<Longrightarrow> \<Sigma> :\<^sub>c t \<Longrightarrow> iter (\<leadsto>\<^sub>t) (encode_state \<Sigma>) (encode_state \<Sigma>')"
 proof (induction \<Sigma> \<Sigma>' rule: evalc.induct)
   case (evc_var cs x c s)
   then obtain t' ts where "(s :\<^sub>c t' \<rightarrow> t) \<and> (cs :\<^sub>c\<^sub>l\<^sub>s ts) \<and> latest_environment s = Some cs \<and> 
     lookup ts x = Some t'" by fastforce
-  then obtain envs where "envs_from_stack s = map compile_closure cs # envs" 
+  then obtain envs where "envs_from_stack s = map encode_closure cs # envs" 
     by (metis lookup_latest)
   with evc_var have "TS (vals_from_stack s) (envs_from_stack s) (TLookup x # code_from_stack s) \<leadsto>\<^sub>t 
-    TS (compile_closure c # vals_from_stack s) (envs_from_stack s) (code_from_stack s)" by simp
+    TS (encode_closure c # vals_from_stack s) (envs_from_stack s) (code_from_stack s)" by simp
   hence "iter (\<leadsto>\<^sub>t) (TS (vals_from_stack s) (envs_from_stack s) (TLookup x # code_from_stack s)) 
-    (TS (compile_closure c # vals_from_stack s) (envs_from_stack s) (code_from_stack s))" 
+    (TS (encode_closure c # vals_from_stack s) (envs_from_stack s) (code_from_stack s))" 
       by (metis iter_step iter_refl)
   thus ?case by simp
 next
@@ -377,40 +381,40 @@ next
   case (evc_lam s cs tt e)
   then obtain t' ts where "(s :\<^sub>c t' \<rightarrow> t) \<and> (cs :\<^sub>c\<^sub>l\<^sub>s ts) \<and> latest_environment s = Some cs \<and>
     (ts \<turnstile>\<^sub>d DLam tt e : t')" by fastforce
-  then obtain envs where "envs_from_stack s = map compile_closure cs # envs" 
+  then obtain envs where "envs_from_stack s = map encode_closure cs # envs" 
     by (metis lookup_latest)
-  hence "TS (vals_from_stack s) (envs_from_stack s) (TPushLam (compile e) # code_from_stack s) \<leadsto>\<^sub>t 
-    TS (TLam (map compile_closure cs) (compile e) # vals_from_stack s) (envs_from_stack s) 
+  hence "TS (vals_from_stack s) (envs_from_stack s) (TPushLam (encode e) # code_from_stack s) \<leadsto>\<^sub>t 
+    TS (TLam (map encode_closure cs) (encode e) # vals_from_stack s) (envs_from_stack s) 
       (code_from_stack s)" by simp
-  hence "iter (\<leadsto>\<^sub>t) (TS (vals_from_stack s) (envs_from_stack s) (TPushLam (compile e) # 
-    code_from_stack s)) (TS (TLam (map compile_closure cs) (compile e) #
+  hence "iter (\<leadsto>\<^sub>t) (TS (vals_from_stack s) (envs_from_stack s) (TPushLam (encode e) # 
+    code_from_stack s)) (TS (TLam (map encode_closure cs) (encode e) #
       vals_from_stack s) (envs_from_stack s) (code_from_stack s))" by (metis iter_step iter_refl)
-  thus ?case by (simp add: compile_def)
+  thus ?case by (simp add: encode_def)
 next
   case (retc_app2 t cs e\<^sub>1 s c\<^sub>2)
-  have "iter (\<leadsto>\<^sub>t) (TS (compile_closure c\<^sub>2 # TLam (map compile_closure cs) 
-    (compile e\<^sub>1) # vals_from_stack s) (envs_from_stack s) (TApply # code_from_stack s))
-      (TS (vals_from_stack s) ((compile_closure c\<^sub>2 # map compile_closure cs) # envs_from_stack s) 
-      (compile e\<^sub>1 @ code_from_stack s))" by (metis evt_apply iter_step iter_refl)
-  thus ?case by (simp add: compile_def)
+  have "iter (\<leadsto>\<^sub>t) (TS (encode_closure c\<^sub>2 # TLam (map encode_closure cs) 
+    (encode e\<^sub>1) # vals_from_stack s) (envs_from_stack s) (TApply # code_from_stack s))
+      (TS (vals_from_stack s) ((encode_closure c\<^sub>2 # map encode_closure cs) # envs_from_stack s) 
+      (encode e\<^sub>1 @ code_from_stack s))" by (metis evt_apply iter_step iter_refl)
+  thus ?case by (simp add: encode_def)
 next
   case (retc_ret cs s c)
-  have "TS (compile_closure c # vals_from_stack s) (map compile_closure cs # envs_from_stack s) 
-    (TReturn # code_from_stack s) \<leadsto>\<^sub>t TS (compile_closure c # vals_from_stack s) (envs_from_stack s) 
+  have "TS (encode_closure c # vals_from_stack s) (map encode_closure cs # envs_from_stack s) 
+    (TReturn # code_from_stack s) \<leadsto>\<^sub>t TS (encode_closure c # vals_from_stack s) (envs_from_stack s) 
       (code_from_stack s)" by simp
-  hence "iter (\<leadsto>\<^sub>t) (TS (compile_closure c # vals_from_stack s) 
-    (map compile_closure cs # envs_from_stack s) (TReturn # code_from_stack s)) 
-      (TS (compile_closure c # vals_from_stack s) (envs_from_stack s) (code_from_stack s))" 
+  hence "iter (\<leadsto>\<^sub>t) (TS (encode_closure c # vals_from_stack s) 
+    (map encode_closure cs # envs_from_stack s) (TReturn # code_from_stack s)) 
+      (TS (encode_closure c # vals_from_stack s) (envs_from_stack s) (code_from_stack s))" 
         by (metis iter_step iter_refl)
   thus ?case by simp
 qed simp_all
 
 lemma iter_completet [simp]: "iter (\<leadsto>\<^sub>c) \<Sigma> \<Sigma>' \<Longrightarrow> \<Sigma> :\<^sub>c t \<Longrightarrow>
-  iter (\<leadsto>\<^sub>t) (compile_state \<Sigma>) (compile_state \<Sigma>')"
+  iter (\<leadsto>\<^sub>t) (encode_state \<Sigma>) (encode_state \<Sigma>')"
 proof (induction \<Sigma> \<Sigma>' rule: iter.induct)
   case (iter_step \<Sigma> \<Sigma>' \<Sigma>'')
-  hence "iter (\<leadsto>\<^sub>t) (compile_state \<Sigma>) (compile_state \<Sigma>')" by simp
-  moreover from iter_step have "iter (\<leadsto>\<^sub>t) (compile_state \<Sigma>') (compile_state \<Sigma>'')" by simp
+  hence "iter (\<leadsto>\<^sub>t) (encode_state \<Sigma>) (encode_state \<Sigma>')" by simp
+  moreover from iter_step have "iter (\<leadsto>\<^sub>t) (encode_state \<Sigma>') (encode_state \<Sigma>'')" by simp
   ultimately show ?case by (metis iter_append)
 qed simp_all
 
