00Utils/Iteration.thy
@@ -6,6 +6,9 @@ inductive iter :: "('a \<Rightarrow> 'a \<Rightarrow> bool) \<Rightarrow> 'a \<R
   iter_refl [simp]: "iter f a a"
 | iter_step [simp]: "f a b \<Longrightarrow> iter f b c \<Longrightarrow> iter f a c"
 
+lemma iter_one: "f a b \<Longrightarrow> iter f a b"
+  by (metis iter_refl iter_step)
+
 lemma iter_append: "iter f a b \<Longrightarrow> iter f b c \<Longrightarrow> iter f a c"
   by (induction a b rule: iter.induct) simp_all
 
